Name magic constants
Add VERSION_1 and TYPE_CUSTOMER_AED.
Change base type of Version and Type to uint8.
Add conversion functions ContentTypeToUInt8 and UInt8ToContentType, and an associated correctness lemma.

src/SDK/MessageHeader/Definitions.dfy
@@ -16,12 +16,39 @@ module MessageHeader.Definitions {
   /*
    * Header body type definition
    */
-  type Version               = x | x == 0x01 /*Version 1.0*/ witness 0x01
-  type Type                  = x | x == 0x80 /*Customer Authenticated Encrypted Data*/ witness 0x80
+  const VERSION_1: uint8     := 0x01
+  type Version               = x | x == VERSION_1 witness VERSION_1
+
+  const TYPE_CUSTOMER_AED: uint8 := 0x80
+  type Type                  = x | x == TYPE_CUSTOMER_AED witness TYPE_CUSTOMER_AED
+
   const MESSAGE_ID_LEN       := 16
   type MessageID             = x: seq<uint8> | |x| == MESSAGE_ID_LEN witness [0,0,0,0,0,0,0,0,0,0,0,0,0,0,0,0]
+
   type Reserved              = x: seq<uint8> | x == [0,0,0,0] witness [0,0,0,0]
+
   datatype ContentType       = NonFramed | Framed
+
+  function method ContentTypeToUInt8(contentType: ContentType): uint8 {
+    match contentType
+    case NonFramed => 0x01
+    case Framed => 0x02
+  }
+
+  function method UInt8ToContentType(x: uint8): Option<ContentType> {
+    if x == 0x01 then
+      Some(NonFramed)
+    else if x == 0x02 then
+      Some(Framed)
+    else
+      None
+  }
+
+  lemma ContentTypeConversionsCorrect(contentType: ContentType, x: uint8)
+    ensures UInt8ToContentType(ContentTypeToUInt8(contentType)) == Some(contentType)
+    ensures var opt := UInt8ToContentType(x); opt == None || ContentTypeToUInt8(opt.get) == x
+  {
+  }
 
   datatype EncryptedDataKeys = EncryptedDataKeys(entries: seq<Materials.EncryptedDataKey>)
 
